# 启发性例题

## #1

求：
$$
\lim _{x \rightarrow+\infty} \sqrt{x}(\sqrt{x+2}-2 \sqrt{x+1}+\sqrt{x})
$$
原式
$$
\begin{align}
 & =\lim _{x \rightarrow+\infty} \sqrt{x}(\sqrt{x+2}-\sqrt{x+1})-\sqrt{x}(\sqrt{x+1}-\sqrt{x})
\\ & =\lim _{x \rightarrow+\infty} \frac{\sqrt{x}}{(\sqrt{x+2}+\sqrt{x+1})}-\lim _{x \rightarrow+\infty} \frac{\sqrt{x}}{(\sqrt{x+2}+\sqrt{x+1})}\\
& =\lim _{x \rightarrow+\infty} \frac{1}{(\sqrt{1+\frac{2}{x}}+\sqrt{1+\frac{1}{x}}}-\lim _{x \rightarrow+\infty} \frac{1}{(\sqrt{1+\frac{1}{x}}+\sqrt{1}}\\
&=\frac{1}{2}-\frac{1}{2}=0
\end{align}
$$

## #2

结论：
$$
\lim_{x\to x_0}u^v=e^{\lim\limits_{x\to x_0}(u-1)v}
$$
证明：
$$
\lim u^v=\lim \left\{[1+(u-1)]^\frac1{u-1}\right\}^{(u-1)v}=e^{\lim(u-1)v}
$$
